Refactor a lot

theories/Alpha/RenameApart_Liveness.v
@@ -2,6 +2,7 @@ Require Import Util CSet Map LengthEq.
 Require Import Env IL Alpha StableFresh Subset1 OptionR.
 Require Import Annotation AnnP RenamedApart RenameApart SetOperations Take.
 Require Import LabelsDefined PairwiseDisjoint Liveness.Liveness Coherence Restrict.
+Require Import FreshGen.
 
 Set Implicit Arguments.
 
@@ -33,130 +34,146 @@ Proof.
     rewrite <- Incl. clear; cset_tac.
 Qed.
 
-Definition renameApartF_live (fresh:StableFresh)
-           (renameApart_live:StableFresh -> env var -> set var -> stmt -> ann (set var) -> set var * ann (set var)) G ϱ :=
-  (fix f (N:set var) (F:list (params*stmt)) (anF:list (ann (set var))) :=
+Definition renameApartF_live {Fi} (FG:FreshGen Fi)
+           (renameApart_live: FreshGen Fi -> Fi -> env var -> stmt -> ann (set var) -> Fi * ann (set var))
+           ϱ :=
+  (fix f fi (F:list (params*stmt)) (anF:list (ann (set var))) :=
      match F, anF with
      | Zs::F, a::anF =>
-       let Y := fst (fresh_list_stable fresh (N ∪ G) (fst Zs)) in
+       let (Y, fi) := fresh_list FG fi (fst Zs) in
        let ϱZ := ϱ [ fst Zs <-- Y ] in
-       let (N', alv') := renameApart_live fresh ϱZ (G ∪ N ∪ of_list Y) (snd Zs) a in
-       let (anF', N'') := f (N' ∪ of_list Y ∪ N) F anF in
-       (setTopAnn alv' (getAnn alv' ∪ of_list Y)::anF', N'')
-     | _, _ => (nil, N)
+       let '(fi, alv') := renameApart_live FG fi ϱZ (snd Zs) a in
+       let (YL, fi) := f fi F anF in
+       (setTopAnn alv' (getAnn alv' ∪ of_list Y)::YL, fi)
+     | _, _ => (nil, fi)
      end).
 
 
-Fixpoint renameApart_live (fresh:StableFresh) (ϱ:env var) (G:set var) (s:stmt) (alv:ann (set var))
-  : set var * ann (set var) :=
+Fixpoint renameApart_live {Fi} (FG:FreshGen Fi) fi
+         (ϱ:env var) (s:stmt) (alv:ann (set var))
+  : Fi * ann (set var) :=
   match s, alv with
   | stmtLet x e s0, ann1 lv alv =>
-    let y := fresh G x in
+    let (y,fi) := fresh FG fi x in
     let ϱ' := ϱ[x <- y] in
-    let (G', alv') := renameApart_live fresh ϱ' {y; G} s0 alv in
-    ({y; G'}, ann1 (lookup_set ϱ lv) alv')
+    let (fi, alv') := renameApart_live FG fi ϱ' s0 alv in
+    (fi, ann1 (lookup_set ϱ lv) alv')
   | stmtIf e s1 s2, ann2 lv alv1 alv2 =>
-    let (G', alv1') := renameApart_live fresh ϱ G s1 alv1 in
-    let (G'', alv2') := renameApart_live fresh ϱ (G ∪ G') s2 alv2 in
-    (G' ∪ G'', ann2 (lookup_set ϱ lv) alv1' alv2')
-  | stmtApp l Y, ann0 lv => (∅, ann0 (lookup_set ϱ lv))
-  | stmtReturn e, ann0 lv => (∅, ann0 (lookup_set ϱ lv))
+    let (fi, alv1') := renameApart_live FG fi ϱ s1 alv1 in
+    let (fi, alv2') := renameApart_live FG fi ϱ s2 alv2 in
+    (fi, ann2 (lookup_set ϱ lv) alv1' alv2')
+  | stmtApp l Y, ann0 lv => (fi, ann0 (lookup_set ϱ lv))
+  | stmtReturn e, ann0 lv => (fi, ann0 (lookup_set ϱ lv))
   | stmtFun F s2, annF lv anF alv2 =>
-    let (anF', G') := renameApartF_live fresh renameApart_live G ϱ ∅ F anF in
-    let (G'', alv2') := renameApart_live fresh ϱ (G ∪ G') s2 alv2 in
-    (G' ∪ G'', annF (lookup_set ϱ lv) anF' alv2')
-  | _ , _ => (∅, alv)
+    let (anF', fi) := renameApartF_live FG renameApart_live ϱ fi F anF in
+    let (fi, alv2') := renameApart_live FG fi ϱ s2 alv2 in
+    (fi, annF (lookup_set ϱ lv) anF' alv2')
+  | _ , _ => (fi, alv)
   end.
 
-Lemma getAnn_snd_renameApart_live fresh o ZL LV ϱ G s lv
+Lemma getAnn_snd_renameApart_live {Fi} (FG:FreshGen Fi) fi o ZL LV ϱ s lv
   : live_sound o ZL LV s lv
-    -> getAnn (snd (renameApart_live fresh ϱ G s lv)) = lookup_set ϱ (getAnn lv).
+    -> getAnn (snd (renameApart_live FG fi ϱ s lv)) = lookup_set ϱ (getAnn lv).
 Proof.
   intros LS; inv LS; simpl; repeat let_pair_case_eq; simpl; subst; eauto.
 Qed.
 
 
-Lemma snd_renameApartF_live fresh als L X G ϱ F (Len:❬F❭ = ❬als❭)
-      (IH:forall n Zs a, get F n Zs -> get als n a ->
+Lemma snd_renameApartF_live' {Fi} (FG:FreshGen Fi) fi als L X ϱ F (Len:❬F❭ = ❬als❭)
+      (IH:forall n Zs a fi, get F n Zs -> get als n a ->
                     forall (ϱ : env var) (G : ⦃var⦄),
-                      fst (renameApart_live fresh ϱ G (snd Zs) a) = fst (renameApart' fresh ϱ G (snd Zs)))
-  : snd (renameApartF_live fresh renameApart_live G ϱ X F als) =
-    snd (renameApartF fresh renameApart' G ϱ F (L, X)).
+                      fst (renameApart_live FG fi ϱ (snd Zs) a) =
+                      snd (fst (renameApart' FG fi ϱ (snd Zs))))
+  : snd (renameApartF_live FG renameApart_live ϱ fi F als) =
+    snd (fst (renameApartF FG renameApart' ϱ F (L, fi, X))).
 Proof.
   length_equify.
   general induction Len.
   - eauto.
-  - simpl. repeat let_pair_case_eq;simpl; subst.
-    unfold renameApartFStep.
-    repeat let_pair_case_eq; simpl; subst; eauto. simpl.
+  - simpl. repeat let_pair_case_eq; simpl; subst; simpl.
     erewrite <- IHLen; eauto using get.
     erewrite <- IH; eauto using get.
 Qed.
 
 
-Lemma fst_renameApart_live fresh o ZL LV ϱ G s lv
+Lemma fst_renameApart_live {Fi} (FG:FreshGen Fi) fi o ZL LV ϱ s lv
   : live_sound o ZL LV s lv
-    -> fst (renameApart_live fresh ϱ G s lv) = fst (renameApart' fresh ϱ G s).
+    -> fst (renameApart_live FG fi ϱ s lv) = snd (fst (renameApart' FG fi ϱ s)).
 Proof.
   intros LS.
   general induction LS; simpl; repeat let_pair_case_eq; simpl; subst; eauto.
-  - rewrite IHLS; eauto.
   - rewrite IHLS1, IHLS2; eauto.
-  - erewrite snd_renameApartF_live; eauto.
-    f_equal; eauto.
+  - erewrite snd_renameApartF_live'; eauto.
+Qed.
+
+Lemma snd_renameApartF_live {Fi} (FG:FreshGen Fi) fi als L X ϱ F (Len:❬F❭ = ❬als❭) ZL Lv i
+      (LS:forall (n : nat) (Zs : params * stmt) (a : ann ⦃nat⦄),
+            get F n Zs ->
+            get als n a -> live_sound i ZL Lv (snd Zs) a)
+  : snd (renameApartF_live FG renameApart_live ϱ fi F als) =
+    snd (fst (renameApartF FG renameApart' ϱ F (L, fi, X))).
+Proof.
+  eapply snd_renameApartF_live'; eauto.
+  intros.
+  eapply fst_renameApart_live; eauto.
 Qed.
 
 
-Lemma renameApartF_live_length fresh G G' ϱ F anF (Len:❬F❭ = ❬anF❭)
-: length (fst (renameApartF_live fresh renameApart_live G ϱ G' F anF)) = length F.
+Lemma renameApartF_live_length {Fi} (FG:FreshGen Fi) fi ϱ F anF (Len:❬F❭ = ❬anF❭)
+: length (fst (renameApartF_live FG renameApart_live ϱ fi F anF)) = length F.
 Proof.
-  length_equify.
   general induction Len; simpl; repeat let_pair_case_eq; simpl; subst; eauto.
 Qed.
 
 Smpl Add match goal with
-         | [ H : context [ ❬fst (renameApartF_live ?fresh ?renameApart' ?G ?ϱ ?s ?F ?anF)❭ ] |- _ ] =>
-           rewrite (@renameApartF_live_length fresh G s ϱ F anF) in H
-         | [ |- context [ ❬fst (renameApartF_live ?fresh ?renameApart' ?G ?ϱ ?s ?F ?anF)❭ ] ] =>
-           rewrite (@renameApartF_live_length fresh G s ϱ F anF)
+         | [ H : context [ ❬fst (renameApartF_live ?FG ?renameApart' ?ϱ ?fi ?F ?anF)❭ ] |- _ ] =>
+           rewrite (@renameApartF_live_length _ FG fi ϱ F anF) in H
+         | [ |- context [ ❬fst (renameApartF_live ?FG ?renameApart' ?ϱ ?fi ?F ?anF)❭ ] ] =>
+           rewrite (@renameApartF_live_length _ FG fi ϱ F anF)
          end : len.
 
-Lemma get_fst_renameApartF_live fresh G G' ϱ F n anF ans
-  (Get: get (fst (renameApartF_live fresh renameApart_live G ϱ G' F anF)) n ans)
+Lemma get_fst_renameApartF_live {Fi} (FG:FreshGen Fi) fi  ϱ F n anF ans
+  (Get: get (fst (renameApartF_live FG renameApart_live ϱ fi F anF)) n ans)
   (Len:❬F❭=❬anF❭)
-  :  exists Zs a  G'' (Y:list var) ans',
+  :  exists Zs a Yfi ans',
     get F n Zs /\ get anF n a
-    /\ ans' = snd (renameApart_live fresh (ϱ [fst Zs <-- Y]) G'' (snd Zs) a) /\
-    ans = setTopAnn ans' (getAnn ans' ∪ of_list Y)/\
-    G'' = G ∪ snd (renameApartF_live fresh renameApart_live G ϱ G' (take n F) (take n anF))
-            ∪ of_list Y
-    /\ Y = (fresh_list_stable fresh (snd (renameApartF_live fresh renameApart_live G ϱ G' (take n F) (take n anF)) ∪ G) (fst Zs)).
+    /\ ans' = snd (renameApart_live FG (snd Yfi) (ϱ [fst Zs <-- fst Yfi]) (snd Zs) a) /\
+    ans = setTopAnn ans' (getAnn ans' ∪ of_list (fst Yfi)) /\
+(*    fi'' = snd (renameApartF_live FG renameApart_live ϱ (snd Yfi) (take n F) (take n anF))*)
+    Yfi = (fresh_list FG (snd (renameApartF_live FG renameApart_live ϱ fi (take n F) (take n anF))) (fst Zs)).
 Proof.
-  length_equify.
   general induction Len; simpl in * |- *; [ isabsurd |].
-  - revert Get; let_pair_case_eq; simpl_pair_eqs; subst; intros Get.
-    revert Get; let_pair_case_eq; simpl_pair_eqs; subst; intros Get. simpl in *.
+  - revert Get; repeat let_pair_case_eq; repeat simpl_pair_eqs; subst; intros Get.
     inv Get.
     + eexists x, y; eauto 100 using get.
-    + edestruct IHLen as [? [? ?]]; dcr; subst; eauto 20 using get.
+    + edestruct IHLen as [? [? [? ?]]]; dcr; subst; eauto 20 using get.
       subst.
-      do 5 eexists; split; [| split]; eauto 100 using get.
+      do 4 eexists; split; [| split]; eauto 100 using get.
       split. reflexivity. simpl.
       repeat let_pair_case_eq; repeat simpl_pair_eqs; subst. simpl.
       split.
       reflexivity. split; reflexivity.
 Qed.
 
-Tactic Notation "orewrite" constr(A) "all" :=
+Smpl Add
+     match goal with
+     | [ H : get (fst (renameApartF_live ?FG renameApart_live ?ϱ ?fi ?F ?anF)) ?n ?ans |- _ ] =>
+       eapply get_fst_renameApartF_live in H
+         as [? [? [? [? [? [? [? [? ?]]]]]]]]; eauto; subst
+     end : inv_get.
+
+
+Tactic Notation "orewrite" constr(A) "in *" :=
   let X := fresh "OX" in assert A as X by omega; rewrite X in *; clear X.
 
-Lemma renameApart_live_sound fresh ZL LV ZL' LV' s lv ϱ G
+Lemma renameApart_live_sound {Fi} (FG:FreshGen Fi) (FGS:FreshGenSpec FG)
+      fi ZL LV ZL' LV' s lv ϱ
       (LenZL:❬ZL❭ = ❬ZL'❭) (LenLV:❬LV❭=❬LV'❭)
       (ParamLen:forall n Z Z', get ZL n Z -> get ZL' n Z' -> ❬Z❭ = ❬Z'❭)
   : live_sound Functional ZL LV s lv
     -> live_sound Functional ZL' LV'
-                 (snd (renameApart' fresh ϱ G s))
-                 (snd (renameApart_live fresh ϱ G s lv)).
+                 (snd (renameApart' FG fi ϱ s))
+                 (snd (renameApart_live FG fi ϱ s lv)).
 Proof.
   intros LS.
   general induction LS; simpl; repeat let_pair_case_eq; simpl; subst; eauto.
@@ -181,88 +198,51 @@ Proof.
         -- rewrite !app_length, !map_length, renameApartF_live_length; eauto.
         -- intros; inv_get.
            eapply get_app_cases in H4; destruct H4.
-           ++ rewrite get_app_lt in H5; inv_get; len_simpl.
-             edestruct (get_fst_renameApartF fresh _ _ _ H5)
-               as [? [? ?]]; eauto; dcr.
-             assert (n < ❬F❭) by eauto using get_range.
-             orewrite (❬F❭ - S (❬F❭ - S n) = n) in H9.
-             get_functional; eauto. eauto with len.
+           ++ rewrite get_app_lt in H5; inv_get; len_simpl; inv_get; eauto.
+             rewrite fresh_list_len; eauto.
            ++ dcr. rewrite get_app_ge in H5; eauto with len.
-      * intros. erewrite fst_renameApart_live; eauto.
     + eauto with len.
-    + intros; inv_get.
-      edestruct (get_fst_renameApartF _ _ _ _ H4) as [? [? ?]];
-        eauto; dcr.
-      rewrite H7.
-      edestruct (get_fst_renameApartF_live _ _ _ _ _ _ H5); eauto; dcr; subst.
-      rewrite renameApartF_length in H8.
-      assert (n < ❬F❭) by eauto using get_range.
-      orewrite (❬F❭ - S (❬F❭ - S n) = n) in H8. get_functional.
-      rewrite H16.
+    + intros; inv_get; len_simpl; inv_get.
       rewrite drop_rev.
       rewrite renameApartFRight_corr.
-      erewrite <- snd_renameApartF_live.
-      rewrite renameApartF_length. rewrite rev_rev. rewrite rev_length.
-      assert (n < ❬F❭) by eauto using get_range.
-      orewrite (❬F❭ - S (❬F❭ - S n) = n).
+      erewrite <- snd_renameApartF_live. len_simpl.
+      orewrite (❬F❭ - S (❬F❭ - S n) = n). rewrite rev_rev.
       eapply live_sound_monotone2.
       eapply H1; eauto.
       revert LenZL; clear; eauto with len.
       revert H LenLV; clear; eauto with len.
       -- intros ? ? ? GetA GetB; inv_get.
-         eapply get_app_cases in GetA; destruct GetA.
-         ++ rewrite get_app_lt in GetB; inv_get.
-           edestruct (get_fst_renameApartF _ _ _ _ GetB) as [? [? ?]];
-             eauto; dcr. subst.
-           rewrite renameApartF_length in H21.
-           assert (n0 < ❬F❭) by eauto using get_range.
-           orewrite (❬F❭ - S (❬F❭ - S n0) = n0) in H21. get_functional. eauto.
-           rewrite map_length, rev_length, renameApartF_length; eauto using get_range.
-         ++ dcr. rewrite get_app_ge in GetB; eauto with len.
+         eapply get_app_cases in GetA as [?|[? ?]].
+         ++ rewrite get_app_lt in GetB; inv_get. len_simpl. inv_get.
+           rewrite fresh_list_len; eauto.
+           eauto with len.
+         ++ rewrite get_app_ge in GetB; eauto with len.
       -- eauto with cset.
-      -- rewrite rev_length, renameApartF_length, rev_rev.
-         assert (n < ❬F❭) by eauto using get_range.
-         orewrite (❬F❭ - S (❬F❭ - S n) = n).
-         repeat rewrite take_length_le; eauto; omega.
-      -- intros. inv_get. len_simpl.
-         assert (n0 < ❬F❭) by eauto using get_range.
-         orewrite (❬F❭ - S (❬F❭ - S n0) = n0) all.
+      -- len_simpl.
+         orewrite (❬F❭ - S (❬F❭ - S n) = n). eauto with len.
+      -- intros. inv_get. len_simpl. inv_get.
          exploit H0; try eapply H15; eauto.
-         erewrite fst_renameApart_live; eauto.
-    + intros ? ? ? GetA GetB; inv_get; simpl.
-      edestruct (get_fst_renameApartF _ _ _ _ GetA) as [? [? ?]];
-        eauto; dcr; subst.
-      rewrite H14.
-      edestruct (get_fst_renameApartF_live _ _ _ _ _ _ GetB);
-        eauto; dcr; subst.
+    + intros ? ? ? GetA GetB; inv_get. len_simpl. inv_get.
       erewrite getAnn_snd_renameApart_live; eauto.
-      exploit H2; eauto; dcr. simpl in H19.
-      rewrite renameApartF_length in H6.
-      assert (n < ❬F❭) by eauto using get_range.
-      orewrite (❬F❭ - S (❬F❭ - S n) = n) in H6.
-      get_functional.
-      rewrite renameApartF_length.
+      exploit H2; eauto. destruct H6 as [? [? ?]].
       rewrite drop_rev.
-      rewrite rev_rev. rewrite rev_length.
-      assert (n < ❬F❭) by eauto using get_range.
+      rewrite renameApartFRight_corr. len_simpl.
       orewrite (❬F❭ - S (❬F❭ - S n) = n).
-      rewrite renameApartFRight_corr.
-      erewrite <- (@snd_renameApartF_live _ (take n als)).
+      rewrite rev_rev.
+      erewrite <- (@snd_renameApartF_live _ FG fi (take n als)).
       split.
       rewrite getAnn_setTopAnn. eauto with cset.
       rewrite getAnn_setTopAnn.
       split.
-      eapply fresh_list_stable_nodup; eauto.
+      eapply fresh_list_nodup; eauto. simpl in *.
       rewrite lookup_set_update_with_list_in_union_length; eauto.
-      rewrite H19. clear. cset_tac. eauto with len.
-      rewrite take_length; eauto with len.
-      -- intros. inv_get.
-         exploit H0; eauto.
-         erewrite fst_renameApart_live; eauto.
+      rewrite <- H8. clear. cset_tac.
+      rewrite fresh_list_len; eauto with len. eauto with len.
+      intros; inv_get; eauto.
     + erewrite getAnn_snd_renameApart_live; eauto with cset.
 Qed.
 
-Lemma renameApart_live_sound_srd b fresh o DL ZL LV (ZL':list params) LV' s lv ϱ G
+Lemma renameApart_live_sound_srd b {Fi} (FG:FreshGen Fi) (FGS:FreshGenSpec FG) fi o DL ZL LV (ZL':list params) LV' s lv ϱ
       (ParamLen:forall n Z Z', get ZL n Z -> get ZL' n Z' -> ❬Z❭ = ❬Z'❭)
   (LS: live_sound o ZL LV s lv)
   (SRD:srd DL s lv)
@@ -270,8 +250,9 @@ Lemma renameApart_live_sound_srd b fresh o DL ZL LV (ZL':list params) LV' s lv �
   (iEQ':PIR2 (ifFstR Equal) (option_map (fun (s:set var) => map ϱ s) ⊝ DL) (LV' \\ ZL'))
   (NUC:noUnreachableCode (isCalled b) s)
   (LenZL:❬ZL❭ = ❬ZL'❭) (LenLV:❬LV❭=❬LV'❭) (LenDL:❬DL❭=❬ZL❭) (LenLV2:❬LV❭=❬ZL❭)
-  (Incl:map ϱ (getAnn lv) ⊆ G) (isImp:isImperative o)
-  : live_sound o ZL' LV' (snd (renameApart' fresh ϱ G s)) (snd (renameApart_live fresh ϱ G s lv)).
+  (Incl:map ϱ (getAnn lv) ⊆ domain FG fi) (isImp:isImperative o)
+  : live_sound o ZL' LV' (snd (renameApart' FG fi ϱ s))
+               (snd (renameApart_live FG fi ϱ s lv)).
 Proof.
   general induction LS; invt srd; invt noUnreachableCode; simpl;
     repeat let_pair_case_eq; simpl; subst; eauto.
@@ -283,18 +264,21 @@ Proof.
         econstructor. rewrite <- H11. revert COND; clear.
         cset_tac'. lud; cset_tac'. eexists x0; lud; eauto.
       * len_simpl. rewrite min_l; try omega.
-      * simpl in *. rewrite <- Incl at 3.
-        revert H0; clear; cset_tac'; lud; eauto.
+      * simpl in *. rewrite <- fresh_domain_spec; eauto.
+        rewrite <- Incl.
+        revert H0; clear_all; cset_tac'; lud; eauto.
     + erewrite getAnn_snd_renameApart_live; eauto.
       rewrite lookup_set_update_union_minus_single; eauto.
       rewrite <- H0. eauto with cset.
     + erewrite getAnn_snd_renameApart_live; eauto.
-      lset_tac. eexists x; lud; eauto.
+      revert H1. clear_all. lset_tac. eexists x; lud; eauto.
   - simpl in *.
     econstructor; eauto using live_op_rename_sound, restrict_ifFstR.
     + eapply IHLS1; eauto with cset.
     + erewrite fst_renameApart_live; eauto.
-      eapply IHLS2; eauto with cset.
+      eapply IHLS2; eauto.
+      rewrite <- renameApart'_domain; eauto.
+      rewrite <- Incl. eauto with cset.
     + erewrite getAnn_snd_renameApart_live; eauto with cset.
     + erewrite getAnn_snd_renameApart_live; eauto with cset.
   - inv_get. exploit ParamLen; eauto.
@@ -309,103 +293,82 @@ Proof.
     + erewrite snd_renameApartF_live; eauto.
       * eapply IHLS; eauto using restrict_ifFstR.
         -- intros; inv_get.
-           eapply get_app_cases in H4; destruct H4.
-           ++ rewrite get_app_lt in H5; inv_get.
-             edestruct (get_fst_renameApartF _ _ _ _ H5) as [? [? ?]]; eauto; dcr.
-             rewrite renameApartF_length in H14.
-             assert (n < ❬F❭) by eauto using get_range.
-             orewrite (❬F❭ - S (❬F❭ - S n) = n) in H14. get_functional. eauto.
-             rewrite map_length, rev_length, renameApartF_length;
-               eauto using get_range.
-           ++ dcr. rewrite get_app_ge in H5; eauto with len.
+           eapply get_app_cases in H4 as [?|[? ?]].
+           ++ rewrite get_app_lt in H5; inv_get. len_simpl; inv_get.
+             rewrite fresh_list_len; eauto.
+             eauto with len.
+           ++ rewrite get_app_ge in H5; eauto with len.
         -- rewrite zip_app;[| eauto with len].
            eauto using PIR2_app, PIR2_ifFstR_refl.
         -- rewrite !zip_app, List.map_app;[| eauto with len].
            apply PIR2_app; eauto with len.
-           eapply PIR2_get; intros; inv_get; simpl; [|eauto with len].
-           econstructor. len_simpl. destruct x2 as [Z s], x as [Z' s'].
+           eapply PIR2_get; intros; inv_get; [|eauto with len].
+           len_simpl. inv_get.
+           econstructor. destruct x as [Z' s'].
            exploit H0; eauto.
-           edestruct (get_fst_renameApartF _ _ _ _ H5) as [? [? ?]]; eauto; dcr.
-           edestruct (get_fst_renameApartF_live _ _ _ _ _ _ H10); eauto; dcr; subst.
-           assert (n < ❬F❭) by eauto using get_range.
-           orewrite (❬F❭ - S (❬F❭ - S n) = n) in H16. get_functional.
-           inv_get.
            rewrite getAnn_setTopAnn. erewrite getAnn_snd_renameApart_live; eauto.
            rewrite drop_rev in *.
            rewrite renameApartFRight_corr in *.
-           simpl in *. subst.
            len_simpl. rewrite rev_rev in *.
-           orewrite (❬F❭ - S (❬F❭ - S n) = n) all.
-           erewrite (snd_renameApartF_live _ nil); eauto;
+           orewrite (❬F❭ - S (❬F❭ - S n) = n).
+           erewrite (snd_renameApartF_live); eauto;
              intros; inv_get; eauto using fst_renameApart_live with len.
            rewrite minus_dist_union.
-           rewrite lookup_set_update_union_minus_list; eauto with len.
+           rewrite lookup_set_update_union_minus_list; eauto with len. simpl.
            setoid_rewrite disj_minus_eq at 2.
            unfold lookup_set. clear; cset_tac.
-           symmetry. eapply disj_2_incl.
-           eapply fresh_list_stable_spec; eauto.
+           symmetry. eapply disj_2_incl. symmetry.
+           eapply fresh_list_disj; eauto.
            exploit H8; eauto.
-           edestruct srd_globals_live_From; eauto; dcr.
+           edestruct srd_globals_live_From as [? [? [? [? ?]]]]; eauto.
            destruct o; simpl in *;
              [ isabsurd | |]; eauto using live_sound_overapproximation_I.
            destruct o; simpl in *;
              [ isabsurd | |]; eauto using live_sound_overapproximation_I.
            inv_get. simpl in *.
-           eapply incl_union_right.
+           rewrite <- domain_incl_renameApartF; eauto.
            rewrite <- Incl. eauto with cset.
+           rewrite fresh_list_len; eauto.
         -- revert LenZL; clear; eauto with len.
         -- revert H LenLV; clear; eauto with len.
         -- revert H LenDL; clear; eauto with len.
         -- revert H LenLV2; clear; eauto with len.
-        -- simpl in *. rewrite <- Incl at 1.
+        -- simpl in *.
+           rewrite <- domain_incl_renameApartF; eauto.
+           rewrite <- Incl.
            eauto with cset.
-      * intros. erewrite fst_renameApart_live; eauto.
     + rewrite rev_length, renameApartF_length, renameApartF_live_length; eauto.
-    + intros; inv_get. len_simpl.
-      edestruct (get_fst_renameApartF _ _ _ _ H4) as [? [? ?]]; eauto; dcr. subst.
-      clear H15 H14.
-      edestruct (get_fst_renameApartF_live _ _ _ _ _ _ H5); eauto; dcr; subst.
-      assert (n < ❬F❭) by eauto using get_range.
-      orewrite (❬F❭ - S (❬F❭ - S n) = n) all. get_functional.
-      rewrite H10, H21.
+    + intros; inv_get. len_simpl. inv_get.
       rewrite drop_rev. rewrite rev_rev. len_simpl.
       orewrite (❬F❭ - S (❬F❭ - S n) = n).
       rewrite renameApartFRight_corr.
-      erewrite <- (@snd_renameApartF_live _ (take n als));
+      erewrite <- (@snd_renameApartF_live _ _ _ (take n als));
         intros; inv_get; eauto using fst_renameApart_live with len.
       eapply live_sound_monotone2.
-      eapply H1; eauto with len.
+      eapply H1; eauto.
       -- intros ? ? ? GetA GetB; inv_get.
-         eapply get_app_cases in GetA; destruct GetA.
-         ++ rewrite get_app_lt in GetB; inv_get.
-           edestruct (get_fst_renameApartF _ _ _ _ GetB) as [? [? ?]];
-             eauto; dcr. subst.
-           len_simpl.
-           assert (n0 < ❬F❭) by eauto using get_range.
-           orewrite (❬F❭ - S (❬F❭ - S n0) = n0) all. get_functional. eauto.
+         eapply get_app_cases in GetA as [?|[? ?]].
+         ++ rewrite get_app_lt in GetB; inv_get; len_simpl; inv_get.
+           rewrite fresh_list_len; eauto.
            eauto with len.
-         ++ dcr. rewrite  get_app_ge in GetB;[|eauto with len ].
+         ++ rewrite get_app_ge in GetB;[|eauto with len ].
            len_simpl.
            exploit ParamLen; eauto.
       -- rewrite !zip_app; eauto with len.
          eauto using PIR2_app, PIR2_ifFstR_refl, restrict_ifFstR.
       -- rewrite !zip_app, !List.map_app; eauto with len.
          apply PIR2_app; eauto with len.
-         ++ eapply PIR2_get; intros; inv_get; simpl; [|eauto with len].
-           repeat cases; simpl; econstructor.
-           len_simpl. destruct x4 as [Z s], x2 as [Z' s'], x0 as [Z'' s''].
-           edestruct (get_fst_renameApartF _ _ _ _ H20) as [? [? ?]]; eauto; dcr.
-           edestruct (get_fst_renameApartF_live _ _ _ _ _ _ H22); eauto; dcr; subst.
-           clear H28 H27.
-           assert (n0 < ❬F❭) by eauto using get_range.
-           orewrite (❬F❭ - S (❬F❭ - S n0) = n0) all. get_functional.
+         ++ eapply PIR2_get; intros; inv_get; [|eauto with len].
+           rewrite getAnn_setTopAnn. simpl restr.
+           repeat cases; eauto; econstructor.
+           len_simpl.
            inv_get.
-           rewrite getAnn_setTopAnn. erewrite getAnn_snd_renameApart_live; eauto.
+           erewrite getAnn_snd_renameApart_live; eauto.
            rewrite drop_rev in *.
-           rewrite renameApartFRight_corr in *. rewrite rev_rev in *.
-           simpl in *. subst. len_simpl.
-           orewrite (❬F❭ - S (❬F❭ - S n0) = n0) all.
-           erewrite <- (@snd_renameApartF_live _ (take n0 als));
+           rewrite renameApartFRight_corr. rewrite rev_rev.
+           len_simpl.
+           orewrite (❬F❭ - S (❬F❭ - S n0) = n0).
+           erewrite (@snd_renameApartF_live _ _ _ (take n0 als));
              intros; inv_get; eauto using fst_renameApart_live with len.
            assert (MME:forall (s t:set var), (t ∪ s) \ s [=] t \ s) by (clear; intros; cset_tac).
            rewrite MME.
@@ -414,22 +377,25 @@ Proof.
            rewrite lookup_set_update_disj; eauto.
            rewrite COND. clear; hnf; cset_tac.
            exploit (H8 n0); eauto.
-           edestruct srd_globals_live_From; eauto; dcr.
+           edestruct srd_globals_live_From as [? [? [? [? ?]]]]; eauto.
            destruct o; simpl in *;
              [ isabsurd | |]; eauto using live_sound_overapproximation_I.
            destruct o; simpl in *;
              [ isabsurd | |]; eauto using live_sound_overapproximation_I.
            inv_get.
-           simpl in *. eapply disj_1_incl. symmetry.
-           eapply fresh_list_stable_spec; eauto.
-           eapply incl_union_right. rewrite <- Incl. eapply map_incl; eauto.
-           rewrite H34; eauto.
+           simpl in *. eapply disj_1_incl.
+           eapply fresh_list_disj; eauto.
+           rewrite <- domain_incl_renameApartF; eauto.
+           rewrite <- Incl. eapply map_incl; eauto.
+           eauto with cset.
+           rewrite fresh_list_len; eauto.
          ++ eapply PIR2_get; intros; inv_get; simpl.
-           ** destruct x; simpl; try now econstructor.
-              unfold restr. cases; simpl; econstructor.
+           ** destruct x1; simpl; try now econstructor.
+              cases; simpl; econstructor.
               rewrite lookup_set_update_disj; eauto.
-              exploit PIR2_nth; try eapply iEQ'; eauto using map_get_eq. dcr.
-              inv_get. simpl in *. inv H28. eauto.
+              exploit PIR2_nth; try eapply iEQ'; eauto using map_get_eq.
+              destruct H16 as [? [? ?]].
+              inv_get. simpl in *. clear_trivial_eqs. eauto.
               rewrite COND. clear; hnf; cset_tac.
            ** len_simpl. exploit PIR2_length; eauto. len_simpl. eauto.
       -- exploit (H8 n); eauto.
@@ -438,37 +404,42 @@ Proof.
            [ isabsurd | |]; eauto using live_sound_overapproximation_I.
          destruct o; simpl in *;
            [ isabsurd | |]; eauto using live_sound_overapproximation_I.
-         rewrite lookup_set_update_with_list_in_union_length; eauto with len.
-         inv_get.
-         rewrite H25. unfold lookup_set. rewrite H3. rewrite Incl.
-         clear; cset_tac.
-      -- eauto with cset.
-    + intros ? ? ? GetA GetB; inv_get; simpl.
-      edestruct (get_fst_renameApartF _ _ _ _ GetA) as [? [? ?]]; eauto; dcr. subst.
-      rewrite H19. len_simpl.
-      edestruct (get_fst_renameApartF_live _ _ _ _ _ _ GetB); eauto; dcr; subst.
+         eauto with len.
+      -- eauto with len.
+      -- eauto with len.
+      -- rewrite <- fresh_list_domain_spec; eauto.
+         rewrite lookup_set_update_with_list_in_union_length.
+         erewrite (@snd_renameApartF_live _ _ _ (take n als));
+           intros; inv_get; eauto using fst_renameApart_live with len.
+         rewrite <- domain_incl_renameApartF; eauto.
+         rewrite union_comm. eapply incl_union_lr; eauto.
+         rewrite <- Incl. simpl.
+         edestruct srd_globals_live_From; eauto.
+          destruct o; simpl in *;
+           [ isabsurd | |]; eauto using live_sound_overapproximation_I.
+         destruct o; simpl in *;
+           [ isabsurd | |]; eauto using live_sound_overapproximation_I.
+         dcr. inv_get. rewrite H15. rewrite <- H3; eauto.
+         eauto. rewrite fresh_list_len; eauto.
+      -- cset_tac.
+    + intros ? ? ? GetA GetB; inv_get. len_simpl. inv_get.
       erewrite getAnn_snd_renameApart_live; eauto.
-      exploit H2; eauto; dcr.
-      assert (n < ❬F❭) by eauto using get_range.
-      orewrite (❬F❭ - S (❬F❭ - S n) = n) all.
-      get_functional.
-      rewrite drop_rev in *.
-      rewrite rev_rev in *. len_simpl.
-      assert (n < ❬F❭) by eauto using get_range.
-      orewrite (❬F❭ - S (❬F❭ - S n) = n) all.
+      exploit H2; eauto. destruct H9 as [? [? ?]].
+      rewrite drop_rev.
+      rewrite rev_rev. len_simpl.
+      orewrite (❬F❭ - S (❬F❭ - S n) = n).
       rewrite renameApartFRight_corr.
-      erewrite <- (@snd_renameApartF_live _ (take n als)).
+      erewrite <- (@snd_renameApartF_live _ _ _ (take n als)).
       split.
       -- rewrite getAnn_setTopAnn. eauto with cset.
       -- split.
-         ++ eapply fresh_list_stable_nodup; eauto.
+         ++ eapply fresh_list_nodup; eauto.
          ++ rewrite getAnn_setTopAnn. cases; eauto.
            rewrite lookup_set_update_with_list_in_union_length; eauto.
-           rewrite H24. clear. cset_tac. eauto with len.
+           rewrite H13. clear. cset_tac.
+           rewrite fresh_list_len; eauto.
       -- eauto with len.
       -- intros. inv_get.
          exploit H0; eauto.
-         erewrite fst_renameApart_live; eauto.
     + erewrite getAnn_snd_renameApart_live; eauto with cset.
 Qed.
-*)
