theories/Constr/CSet.v
@@ -427,11 +427,13 @@ Proof.
   + econstructor; eauto.
 Qed.
 
+(*
 Instance diff_m_eq X `{OrderedType X}
   : Proper (eq ==> eq ==> eq) diff.
 Proof.
   unfold Proper, respectful; intros; subst; eauto.
 Qed.
+
 
 Instance Subset_m_eq_eq_flip_impl X `{OrderedType X}
   : (Proper (eq ==> eq ==> flip impl) Subset).
@@ -439,13 +441,14 @@ Proof.
   unfold Proper, respectful, flip, impl; intros; subst; eauto.
 Qed.
 
+
 Instance Subset_m_Equal_eq_flip_impl X `{OrderedType X}
   : (Proper (Equal ==> eq ==> flip impl) Subset).
 Proof.
   unfold Proper, respectful, flip, impl; intros; subst.
   rewrite H0; eauto.
 Qed.
-
+ *)
 
 Instance prod_eq_fst_morphism X Y R R'
 : Proper (@prod_eq X Y R R' ==> R) fst.
